Done incorporating the empty type
Co-authored-by: Assia Mahboubi <assia.mahboubi@inria.fr>

theories/AutoSubst/PiUniv.sig
@@ -11,3 +11,6 @@ tNat : term
 tZero : term
 tSucc : term -> term
 tNatElim : (bind term in term) -> term -> term -> term -> term
+
+tEmpty : term
+tEmptyElim : (bind term in term) -> term -> term
