theories/AutoSubst/Ast.v
@@ -14,7 +14,9 @@ Inductive term : Type :=
   | tNat : term
   | tZero : term
   | tSucc : term -> term
-  | tNatElim : term -> term -> term -> term -> term.
+  | tNatElim : term -> term -> term -> term -> term
+  | tEmpty : term
+  | tEmptyElim : term -> term -> term.
 
 Lemma congr_tSort {s0 : sort} {t0 : sort} (H0 : s0 = t0) :
   tSort s0 = tSort t0.
@@ -73,6 +75,18 @@ exact (eq_trans
          (ap (fun x => tNatElim t0 t1 t2 x) H3)).
 Qed.
 
+Lemma congr_tEmpty : tEmpty = tEmpty.
+Proof.
+exact (eq_refl).
+Qed.
+
+Lemma congr_tEmptyElim {s0 : term} {s1 : term} {t0 : term} {t1 : term}
+  (H0 : s0 = t0) (H1 : s1 = t1) : tEmptyElim s0 s1 = tEmptyElim t0 t1.
+Proof.
+exact (eq_trans (eq_trans eq_refl (ap (fun x => tEmptyElim x s1) H0))
+         (ap (fun x => tEmptyElim t0 x) H1)).
+Qed.
+
 Lemma upRen_term_term (xi : nat -> nat) : nat -> nat.
 Proof.
 exact (up_ren xi).
@@ -93,6 +107,10 @@ Fixpoint ren_term (xi_term : nat -> nat) (s : term) {struct s} : term :=
   | tNatElim s0 s1 s2 s3 =>
       tNatElim (ren_term (upRen_term_term xi_term) s0) (ren_term xi_term s1)
         (ren_term xi_term s2) (ren_term xi_term s3)
+  | tEmpty => tEmpty
+  | tEmptyElim s0 s1 =>
+      tEmptyElim (ren_term (upRen_term_term xi_term) s0)
+        (ren_term xi_term s1)
   end.
 
 Lemma up_term_term (sigma : nat -> term) : nat -> term.
@@ -119,6 +137,10 @@ term :=
       tNatElim (subst_term (up_term_term sigma_term) s0)
         (subst_term sigma_term s1) (subst_term sigma_term s2)
         (subst_term sigma_term s3)
+  | tEmpty => tEmpty
+  | tEmptyElim s0 s1 =>
+      tEmptyElim (subst_term (up_term_term sigma_term) s0)
+        (subst_term sigma_term s1)
   end.
 
 Lemma upId_term_term (sigma : nat -> term)
@@ -156,6 +178,11 @@ subst_term sigma_term s = s :=
         (idSubst_term sigma_term Eq_term s1)
         (idSubst_term sigma_term Eq_term s2)
         (idSubst_term sigma_term Eq_term s3)
+  | tEmpty => congr_tEmpty
+  | tEmptyElim s0 s1 =>
+      congr_tEmptyElim
+        (idSubst_term (up_term_term sigma_term) (upId_term_term _ Eq_term) s0)
+        (idSubst_term sigma_term Eq_term s1)
   end.
 
 Lemma upExtRen_term_term (xi : nat -> nat) (zeta : nat -> nat)
@@ -195,6 +222,12 @@ ren_term xi_term s = ren_term zeta_term s :=
         (extRen_term xi_term zeta_term Eq_term s1)
         (extRen_term xi_term zeta_term Eq_term s2)
         (extRen_term xi_term zeta_term Eq_term s3)
+  | tEmpty => congr_tEmpty
+  | tEmptyElim s0 s1 =>
+      congr_tEmptyElim
+        (extRen_term (upRen_term_term xi_term) (upRen_term_term zeta_term)
+           (upExtRen_term_term _ _ Eq_term) s0)
+        (extRen_term xi_term zeta_term Eq_term s1)
   end.
 
 Lemma upExt_term_term (sigma : nat -> term) (tau : nat -> term)
@@ -235,6 +268,12 @@ subst_term sigma_term s = subst_term tau_term s :=
         (ext_term sigma_term tau_term Eq_term s1)
         (ext_term sigma_term tau_term Eq_term s2)
         (ext_term sigma_term tau_term Eq_term s3)
+  | tEmpty => congr_tEmpty
+  | tEmptyElim s0 s1 =>
+      congr_tEmptyElim
+        (ext_term (up_term_term sigma_term) (up_term_term tau_term)
+           (upExt_term_term _ _ Eq_term) s0)
+        (ext_term sigma_term tau_term Eq_term s1)
   end.
 
 Lemma up_ren_ren_term_term (xi : nat -> nat) (zeta : nat -> nat)
@@ -278,6 +317,13 @@ Fixpoint compRenRen_term (xi_term : nat -> nat) (zeta_term : nat -> nat)
         (compRenRen_term xi_term zeta_term rho_term Eq_term s1)
         (compRenRen_term xi_term zeta_term rho_term Eq_term s2)
         (compRenRen_term xi_term zeta_term rho_term Eq_term s3)
+  | tEmpty => congr_tEmpty
+  | tEmptyElim s0 s1 =>
+      congr_tEmptyElim
+        (compRenRen_term (upRen_term_term xi_term)
+           (upRen_term_term zeta_term) (upRen_term_term rho_term)
+           (up_ren_ren _ _ _ Eq_term) s0)
+        (compRenRen_term xi_term zeta_term rho_term Eq_term s1)
   end.
 
 Lemma up_ren_subst_term_term (xi : nat -> nat) (tau : nat -> term)
@@ -325,6 +371,12 @@ subst_term tau_term (ren_term xi_term s) = subst_term theta_term s :=
            s0) (compRenSubst_term xi_term tau_term theta_term Eq_term s1)
         (compRenSubst_term xi_term tau_term theta_term Eq_term s2)
         (compRenSubst_term xi_term tau_term theta_term Eq_term s3)
+  | tEmpty => congr_tEmpty
+  | tEmptyElim s0 s1 =>
+      congr_tEmptyElim
+        (compRenSubst_term (upRen_term_term xi_term) (up_term_term tau_term)
+           (up_term_term theta_term) (up_ren_subst_term_term _ _ _ Eq_term)
+           s0) (compRenSubst_term xi_term tau_term theta_term Eq_term s1)
   end.
 
 Lemma up_subst_ren_term_term (sigma : nat -> term) (zeta_term : nat -> nat)
@@ -386,6 +438,13 @@ ren_term zeta_term (subst_term sigma_term s) = subst_term theta_term s :=
         (compSubstRen_term sigma_term zeta_term theta_term Eq_term s1)
         (compSubstRen_term sigma_term zeta_term theta_term Eq_term s2)
         (compSubstRen_term sigma_term zeta_term theta_term Eq_term s3)
+  | tEmpty => congr_tEmpty
+  | tEmptyElim s0 s1 =>
+      congr_tEmptyElim
+        (compSubstRen_term (up_term_term sigma_term)
+           (upRen_term_term zeta_term) (up_term_term theta_term)
+           (up_subst_ren_term_term _ _ _ Eq_term) s0)
+        (compSubstRen_term sigma_term zeta_term theta_term Eq_term s1)
   end.
 
 Lemma up_subst_subst_term_term (sigma : nat -> term) (tau_term : nat -> term)
@@ -449,6 +508,13 @@ subst_term tau_term (subst_term sigma_term s) = subst_term theta_term s :=
         (compSubstSubst_term sigma_term tau_term theta_term Eq_term s1)
         (compSubstSubst_term sigma_term tau_term theta_term Eq_term s2)
         (compSubstSubst_term sigma_term tau_term theta_term Eq_term s3)
+  | tEmpty => congr_tEmpty
+  | tEmptyElim s0 s1 =>
+      congr_tEmptyElim
+        (compSubstSubst_term (up_term_term sigma_term)
+           (up_term_term tau_term) (up_term_term theta_term)
+           (up_subst_subst_term_term _ _ _ Eq_term) s0)
+        (compSubstSubst_term sigma_term tau_term theta_term Eq_term s1)
   end.
 
 Lemma renRen_term (xi_term : nat -> nat) (zeta_term : nat -> nat) (s : term)
@@ -556,6 +622,12 @@ Fixpoint rinst_inst_term (xi_term : nat -> nat) (sigma_term : nat -> term)
         (rinst_inst_term xi_term sigma_term Eq_term s1)
         (rinst_inst_term xi_term sigma_term Eq_term s2)
         (rinst_inst_term xi_term sigma_term Eq_term s3)
+  | tEmpty => congr_tEmpty
+  | tEmptyElim s0 s1 =>
+      congr_tEmptyElim
+        (rinst_inst_term (upRen_term_term xi_term) (up_term_term sigma_term)
+           (rinstInst_up_term_term _ _ Eq_term) s0)
+        (rinst_inst_term xi_term sigma_term Eq_term s1)
   end.
 
 Lemma rinstInst'_term (xi_term : nat -> nat) (s : term) :
@@ -767,6 +839,10 @@ Fixpoint allfv_term (p_term : nat -> Prop) (s : term) {struct s} : Prop :=
       and (allfv_term (upAllfv_term_term p_term) s0)
         (and (allfv_term p_term s1)
            (and (allfv_term p_term s2) (and (allfv_term p_term s3) True)))
+  | tEmpty => True
+  | tEmptyElim s0 s1 =>
+      and (allfv_term (upAllfv_term_term p_term) s0)
+        (and (allfv_term p_term s1) True)
   end.
 
 Lemma upAllfvTriv_term_term {p : nat -> Prop} (H : forall x, p x) :
@@ -806,6 +882,12 @@ Fixpoint allfvTriv_term (p_term : nat -> Prop) (H_term : forall x, p_term x)
         (conj (allfvTriv_term p_term H_term s1)
            (conj (allfvTriv_term p_term H_term s2)
               (conj (allfvTriv_term p_term H_term s3) I)))
+  | tEmpty => I
+  | tEmptyElim s0 s1 =>
+      conj
+        (allfvTriv_term (upAllfv_term_term p_term)
+           (upAllfvTriv_term_term H_term) s0)
+        (conj (allfvTriv_term p_term H_term s1) I)
   end.
 
 Lemma upAllfvImpl_term_term {p : nat -> Prop} {q : nat -> Prop}
@@ -916,6 +998,22 @@ allfv_term p_term s -> allfv_term q_term s :=
                             end
                         end
                     end) I)))
+  | tEmpty => fun HP => I
+  | tEmptyElim s0 s1 =>
+      fun HP =>
+      conj
+        (allfvImpl_term (upAllfv_term_term p_term) (upAllfv_term_term q_term)
+           (upAllfvImpl_term_term H_term) s0
+           match HP with
+           | conj HP _ => HP
+           end)
+        (conj
+           (allfvImpl_term p_term q_term H_term s1
+              match HP with
+              | conj _ HP => match HP with
+                             | conj HP _ => HP
+                             end
+              end) I)
   end.
 
 Lemma upAllfvRenL_term_term (p : nat -> Prop) (xi : nat -> nat) :
@@ -1025,6 +1123,22 @@ allfv_term (funcomp p_term xi_term) s :=
                             end
                         end
                     end) I)))
+  | tEmpty => fun H => I
+  | tEmptyElim s0 s1 =>
+      fun H =>
+      conj
+        (allfvImpl_term _ _ (upAllfvRenL_term_term p_term xi_term) s0
+           (allfvRenL_term (upAllfv_term_term p_term)
+              (upRen_term_term xi_term) s0 match H with
+                                           | conj H _ => H
+                                           end))
+        (conj
+           (allfvRenL_term p_term xi_term s1
+              match H with
+              | conj _ H => match H with
+                            | conj H _ => H
+                            end
+              end) I)
   end.
 
 Lemma upAllfvRenR_term_term (p : nat -> Prop) (xi : nat -> nat) :
@@ -1135,6 +1249,23 @@ allfv_term p_term (ren_term xi_term s) :=
                             end
                         end
                     end) I)))
+  | tEmpty => fun H => I
+  | tEmptyElim s0 s1 =>
+      fun H =>
+      conj
+        (allfvRenR_term (upAllfv_term_term p_term) (upRen_term_term xi_term)
+           s0
+           (allfvImpl_term _ _ (upAllfvRenR_term_term p_term xi_term) s0
+              match H with
+              | conj H _ => H
+              end))
+        (conj
+           (allfvRenR_term p_term xi_term s1
+              match H with
+              | conj _ H => match H with
+                            | conj H _ => H
+                            end
+              end) I)
   end.
 
 End Allfv.
