theories/NormalForms.v
@@ -11,11 +11,13 @@ Inductive whnf : term -> Type :=
   | whnf_tNat : whnf tNat
   | whnf_tZero : whnf tZero
   | whnf_tSucc {n} : whnf (tSucc n)
+  | whnf_tEmpty : whnf tEmpty
   | whnf_whne {n} : whne n -> whnf n
 with whne : term -> Type :=
   | whne_tRel {v} : whne (tRel v)
   | whne_tApp {n t} : whne n -> whne (tApp n t)
-  | whne_tNatElim {P hz hs n} : whne n -> whne (tNatElim P hz hs n).
+  | whne_tNatElim {P hz hs n} : whne n -> whne (tNatElim P hz hs n)
+  | whne_tEmptyElim {P e} : whne e -> whne (tEmptyElim P e).
 
 #[global] Hint Constructors whne whnf : gen_typing.
 
@@ -48,11 +50,13 @@ Inductive isType : term -> Type :=
   | UnivType {s} : isType (tSort s)
   | ProdType { A B} : isType (tProd A B)
   | NatType : isType tNat
+  | EmptyType : isType tEmpty
   | NeType {A}  : whne A -> isType A.
 
 Inductive isPosType : term -> Type :=
   | UnivPos {s} : isPosType (tSort s)
   | NatPos : isPosType tNat
+  | EmptyPos : isPosType tEmpty
   | NePos {A}  : whne A -> isPosType A.
 
 Inductive isFun : term -> Type :=
@@ -63,6 +67,7 @@ Definition isPosType_isType t (i : isPosType t) : isType t :=
   match i with
     | UnivPos => UnivType
     | NatPos => NatType
+    | EmptyPos => EmptyType
     | NePos ne => NeType ne
   end.
 
@@ -73,6 +78,7 @@ Definition isType_whnf t (i : isType t) : whnf t :=
     | UnivType => whnf_tSort
     | ProdType => whnf_tProd
     | NatType => whnf_tNat
+    | EmptyType => whnf_tEmpty
     | NeType ne => whnf_whne ne
   end.
 
