theories/LogicalRelation/Escape.v
@@ -23,6 +23,7 @@ Section Escapes.
     - intros ??? [] **; cbn in *.
       now gen_typing.
     - intros ??? []; gen_typing.
+    - intros ??? []; gen_typing.
   Qed.
 
   Lemma escapeEq {l Γ A B} (lr : [Γ ||-< l > A]) :
@@ -39,6 +40,7 @@ Section Escapes.
     + intros ??? [] * ? ? [] ; cbn in *.
       gen_typing.
     + intros ??? [] []; gen_typing.
+    + intros ??? [] []; gen_typing.
   Qed.
 
   Definition escapeTerm {l Γ t A} (lr : [Γ ||-< l > A ]) :
@@ -52,6 +54,7 @@ Section Escapes.
       gen_typing.
     - intros ??? [] * ?? [] ; cbn in *.
       gen_typing.
+    - intros ??? [] []; gen_typing.
     - intros ??? [] []; gen_typing.
   Qed.
 
@@ -69,6 +72,8 @@ Section Escapes.
     - intros ??? [] * ?? [[termL] [termR]] ; cbn in *.
       eapply convtm_exp ; tea.
       all: gen_typing.
+    - intros ??? [] []; cbn in *.
+      eapply convtm_exp; tea; gen_typing.
     - intros ??? [] []; cbn in *.
       eapply convtm_exp; tea; gen_typing.
   Qed.
